interface; trying to take advantage of reify

examples/layeredeffects/LowParseWriters.fst
@@ -25,83 +25,13 @@ module U8 = FStar.UInt8
 module U32 = FStar.UInt32
 module HST = FStar.HyperStack.ST
 
-assume type parser' (t: Type0) : Type0
+let parser' = admit ()
 
-let parser : Type u#1 = (t: Type0 & parser' t)
+let valid_pos = admit ()
 
-inline_for_extraction
-let dsnd
-  (#u: Type)
-  (#v: ((x: u) -> Type))
-  (p: dtuple2 u v)
-: Tot (v (dfst p))
-= match p with (| _, x |) -> x
+let valid_pos_post = admit ()
 
-assume
-val valid_pos
-  (p: parser)
-  (h: HS.mem)
-  (b: B.buffer U8.t)
-  (pos: U32.t)
-  (pos' : U32.t)
-: GTot Type0
-
-assume
-val valid_pos_post
-  (p: parser)
-  (h: HS.mem)
-  (b: B.buffer U8.t)
-  (pos: U32.t)
-  (pos' : U32.t)
-: Lemma
-  (requires (valid_pos p h b pos pos'))
-  (ensures (
-    B.live h b /\
-    U32.v pos <= U32.v pos' /\
-    U32.v pos' <= B.length b
-  ))
-  [SMTPat (valid_pos p h b pos pos')]
-
-assume
-val contents
-  (p: parser)
-  (h: HS.mem)
-  (b: B.buffer U8.t)
-  (pos: U32.t)
-  (pos' : U32.t)
-: Ghost (dfst p)
-  (requires (valid_pos p h b pos pos'))
-  (ensures (fun _ -> True))
-
-unfold
-let pure_wp_mono
-  (a: Type)
-  (wp: pure_wp a)
-: GTot Type0
-= (forall (p q:pure_post a).
-     (forall (x:a). p x ==> q x) ==> (wp p ==> wp q))
-
-let pre_t
-  (rin: parser)
-: Tot Type
-= dfst rin -> GTot Type0
-
-let post_t
-  (a: Type)
-  (rin: parser)
-  (rout: a -> Tot parser)
-  (pre: pre_t rin)
-: Tot Type
-= (x: dfst rin { pre x }) -> (res: a) -> dfst (rout res) -> GTot Type0
-
-inline_for_extraction
-let repr_spec (a:Type u#x) (r_in: parser) (r_out:a -> parser) (pre: pre_t r_in) (post: post_t a r_in r_out pre) : Tot (Type u#x) =
-  (v_in: dfst r_in) ->
-  Ghost (v: a & dfst (r_out v))
-  (requires (pre v_in))
-  (ensures (fun (| v, v_out |) -> post v_in v v_out))
-
-type u8 : Type0 = U8.t
+let contents = admit ()
 
 unfold
 let repr_impl_post
@@ -136,8 +66,6 @@ let buffer_offset
 : Tot Type0
 = pos1: U32.t { U32.v pos1 <= B.length b }
 
-inline_for_extraction
-unfold
 let repr_impl
   (a:Type u#x)
   (r_in: parser)
@@ -159,78 +87,11 @@ let repr_impl
   ))
 
 inline_for_extraction
-let repr
-  (a: Type u#x)
-  (r_in: parser) (r_out:a -> parser)
-  (pre: pre_t r_in)
-  (post: post_t a r_in r_out pre)
-  (l: B.loc)
-: Tot (Type u#x)
-= dtuple2 (repr_spec a r_in r_out pre post) (repr_impl a r_in r_out pre post l)
-
-unfold
-let return_pre
-  (a:Type) (x:a) (r: a -> parser)
-: Tot (pre_t (r x))
-= fun _ -> True
-
-unfold
-let return_post
-  (a:Type) (x:a) (r: a -> parser)
-: Tot (post_t a (r x) r (return_pre a x r))
-= fun ppre x' ppost -> x' == x /\ ppost == ppre
-
-let return_spec
-  (a:Type) (x:a) (r: a -> parser)
-: Tot (repr_spec a (r x) r (return_pre a x r) (return_post a x r))
-= fun c -> (| x, c |)
-
-inline_for_extraction
 let return_impl
   (a:Type) (x:a) (r: a -> parser)
   (l: B.loc)
 : Tot (repr_impl a (r x) r (return_pre a x r) (return_post a x r) l (return_spec a x r))
 = fun b pos1 -> (x, pos1)
-
-inline_for_extraction
-let returnc
-  (a:Type) (x:a) (r: a -> parser) (l: B.loc)
-: Tot (repr a (r x) r (return_pre a x r) (return_post a x r) l)
-= (| return_spec a x r, return_impl a x r l |)
-
-unfold
-let bind_pre
-  (a:Type) (b:Type)
-  (r_in_f:parser) (r_out_f:a -> parser)
-  (pre_f:pre_t r_in_f) (post_f: post_t a r_in_f r_out_f pre_f)
-  (pre_g: (x:a) ->  pre_t (r_out_f x))
-: Tot (pre_t r_in_f)
-= fun v_in -> pre_f v_in /\ (forall (x: a) v_out . post_f v_in x v_out ==> pre_g x v_out)
-
-unfold
-let bind_post
-  (a:Type) (b:Type)
-  (r_in_f:parser) (r_out_f:a -> parser)
-  (pre_f:pre_t r_in_f) (post_f: post_t a r_in_f r_out_f pre_f)
-  (r_out_g:b -> parser)
-  (pre_g: (x:a) ->  pre_t (r_out_f x))
-  (post_g: (x:a) -> post_t b (r_out_f x) r_out_g (pre_g x))
-: Tot (post_t b r_in_f r_out_g (bind_pre a b r_in_f r_out_f pre_f post_f pre_g))
-= fun v_in y v_out ->
-  exists x v_out_f . pre_f v_in /\ post_f v_in x v_out_f /\ post_g x v_out_f y v_out
-
-let bind_spec (a:Type) (b:Type)
-  (r_in_f:parser) (r_out_f:a -> parser)
-  (pre_f: pre_t r_in_f) (post_f: post_t a r_in_f r_out_f pre_f)
-  (r_out_g:b -> parser)
-  (pre_g: (x:a) -> pre_t (r_out_f x)) (post_g: (x:a) -> post_t b (r_out_f x) r_out_g (pre_g x))
-  (f_bind_spec:repr_spec a r_in_f r_out_f pre_f post_f)
-  (g:(x:a -> repr_spec b (r_out_f x) r_out_g (pre_g x) (post_g x)))
-: Tot (repr_spec b r_in_f r_out_g (bind_pre a b r_in_f r_out_f pre_f post_f pre_g) (bind_post a b r_in_f r_out_f pre_f post_f r_out_g pre_g post_g))
-= fun c ->
-  match f_bind_spec c with
-  | (| x, cf |) ->
-    g x cf
 
 let loc_includes_loc_buffer_loc_buffer_from_to
   (#a: _) (#rrel #rel: _)
@@ -269,283 +130,36 @@ let bind_impl
   | (x, posf) -> g' x buf posf
 
 inline_for_extraction
-let bind (a:Type) (b:Type)
-  (r_in_f:parser) (r_out_f:a -> parser)
-  (pre_f: pre_t r_in_f) (post_f: post_t a r_in_f r_out_f pre_f)
-  (r_out_g:b -> parser)
-  (pre_g: (x:a) -> pre_t (r_out_f x)) (post_g: (x:a) -> post_t b (r_out_f x) r_out_g (pre_g x))
-  (l: B.loc)
-  (f_bind : repr a r_in_f r_out_f pre_f post_f l)
-  (g : (x: a -> repr b (r_out_f x) r_out_g (pre_g x) (post_g x) l))
-: Tot (repr b r_in_f r_out_g (bind_pre a b r_in_f r_out_f pre_f post_f pre_g) (bind_post a b r_in_f r_out_f pre_f post_f r_out_g pre_g post_g) l)
-= (| bind_spec a b r_in_f r_out_f pre_f post_f r_out_g pre_g post_g (dfst f_bind) (fun x -> dfst (g x)), bind_impl a b r_in_f r_out_f pre_f post_f r_out_g pre_g post_g (dfst f_bind) (fun x -> dfst (g x)) l (dsnd f_bind) (fun x -> dsnd (g x)) |)
-
-unfold
-let subcomp_cond
-  (a:Type)
+let subcomp_impl (a:Type)
   (r_in:parser) (r_out:a -> parser)
   (pre: pre_t r_in) (post: post_t a r_in r_out pre)
   (pre': pre_t r_in) (post': post_t a r_in r_out pre')
   (l:B.loc)
   (l' : B.loc)
-: GTot Type0
-= l `B.loc_includes` l' /\
-  (forall v_in . pre' v_in ==> pre v_in) /\
-  (forall v_in x v_out . (pre' v_in /\ post v_in x v_out) ==> post' v_in x v_out)
+  (f_subcomp_spec:repr_spec a r_in r_out pre post)
+  (f_subcomp:repr_impl a r_in r_out pre post l f_subcomp_spec)
+  (sq: squash (subcomp_cond a r_in r_out pre post pre' post' l l'))
+: Tot (repr_impl a r_in r_out pre' post' l' (subcomp_spec a r_in r_out pre post pre' post' f_subcomp_spec))
+= (fun b pos -> f_subcomp b pos)
 
 inline_for_extraction
-let subcomp (a:Type)
-  (r_in:parser) (r_out:a -> parser)
-  (pre: pre_t r_in) (post: post_t a r_in r_out pre)
-  (pre': pre_t r_in) (post': post_t a r_in r_out pre')
-  (l:B.loc)
-  (l' : B.loc)
-  (f_subcomp:repr a r_in r_out pre post l)
-: Pure (repr a r_in r_out pre' post' l')
-  (requires (subcomp_cond a r_in r_out pre post pre' post' l l'))
-  (ensures (fun _ -> True))
-= (| (fun x -> dfst f_subcomp x), (fun pos -> dsnd f_subcomp pos) |)
-
-unfold
-let if_then_else_pre
-  (r_in:parser)
-  (pre_f pre_g: pre_t r_in)
-  (p:Type0)
-: Tot (pre_t r_in)
-= fun v_in -> (p ==> pre_f v_in) /\ ((~ p) ==> pre_g v_in)
-
-unfold
-let if_then_else_post
-  (a:Type)
-  (r_in:parser) (r_out:a -> parser)
-  (pre_f pre_g: pre_t r_in)
-  (post_f: post_t a r_in r_out pre_f)
-  (post_g: post_t a r_in r_out pre_g)
-  (p:Type0)
-: Tot (post_t a r_in r_out (if_then_else_pre r_in pre_f pre_g p))
-= fun v_in x v_out ->
-  (p ==> post_f v_in x v_out) /\
-  ((~ p) ==> post_g v_in x v_out)
-
-let if_then_else (a:Type)
-  (r_in:parser) (r_out:a -> parser)
-  (pre_f pre_g: pre_t r_in)
-  (post_f: post_t a r_in r_out pre_f)
-  (post_g: post_t a r_in r_out pre_g)
-  (l:B.loc)
-  (f_ifthenelse:repr a r_in r_out pre_f post_f l)
-  (g:repr a r_in r_out pre_g post_g l)
-  (p:Type0)
-: Tot Type
-= repr a r_in r_out (if_then_else_pre r_in pre_f pre_g p) (if_then_else_post a r_in r_out pre_f pre_g post_f post_g p) l
-
-#push-options "--print_universes"
-
-reifiable reflectable total
-layered_effect {
-  Write : a:Type -> (pin: parser) -> (pout: (a -> parser)) -> (pre: pre_t pin) -> (post: post_t a pin pout pre) -> (B.loc) -> Effect
-  with
-  repr = repr;
-  return = returnc;
-  bind = bind;
-  subcomp = subcomp;
-  if_then_else = if_then_else
-}
-
-#pop-options
-
-unfold
-let lift_pure_pre
-  (a:Type) (wp:pure_wp a { pure_wp_mono a wp }) (r:parser)
-: Tot (pre_t r)
-= fun st -> wp (fun _ -> True)
-
-unfold
-let lift_pure_post
-  (a:Type) (wp:pure_wp a { pure_wp_mono a wp }) (r:parser)
-: Tot (post_t a r (fun _ -> r) (lift_pure_pre a wp r))
-= fun st x st' -> ~ (wp (fun x' -> ~ (st == st' /\ x == x')))
-
-let lift_pure_spec
-  (a:Type) (wp:pure_wp a { pure_wp_mono a wp }) (r:parser) (f_pure_spec:unit -> PURE a wp)
-: Tot (repr_spec a r (fun _ -> r) (lift_pure_pre a wp r) (lift_pure_post a wp r))
-= fun v -> (| f_pure_spec (), v |)
-
 let lift_pure_impl
   (a:Type) (wp:pure_wp a { pure_wp_mono a wp }) (r:parser) (f_pure_spec_for_impl:unit -> PURE a wp)
   (l: B.loc)
 : Tot (repr_impl a r (fun _ -> r) (lift_pure_pre a wp r) (lift_pure_post a wp r) l (lift_pure_spec a wp r f_pure_spec_for_impl))
 = fun buf pos -> (f_pure_spec_for_impl (), pos)
 
-let lift_pure (a:Type) (wp:pure_wp a { pure_wp_mono a wp }) (r:parser)
-  (l: B.loc)
-  (f_pure:unit -> PURE a wp)
-: Tot (repr a r (fun _ -> r) (lift_pure_pre a wp r) (lift_pure_post a wp r) l)
-= (| lift_pure_spec a wp r f_pure, lift_pure_impl a wp r f_pure l |)
+let emp' = admit ()
 
-sub_effect PURE ~> Write = lift_pure
+let valid_emp = admit ()
 
-inline_for_extraction
-let destr_repr_spec
-  (a:Type u#x)
-  (r_in: parser)
-  (r_out:a -> parser)
-  (pre: pre_t r_in)
-  (post: post_t a r_in r_out pre)
-  (l: B.loc)
-  (f_destr_spec: unit -> Write a r_in r_out pre post l)
-: Tot (repr_spec a r_in r_out pre post)
-= dfst (reify (f_destr_spec ()))
+let star' = admit ()
 
-inline_for_extraction
-let destr_repr_impl
-  (a:Type u#x)
-  (r_in: parser)
-  (r_out:a -> parser)
-  (pre: pre_t r_in)
-  (post: post_t a r_in r_out pre)
-  (l: B.loc)
-  (f_destr_spec: unit -> Write a r_in r_out pre post l)
-: Tot (repr_impl a r_in r_out pre post l (destr_repr_spec a r_in r_out pre post l f_destr_spec))
-= dsnd (reify (f_destr_spec ()))
+let valid_star = admit ()
 
-inline_for_extraction
-let mk_repr
-  (a:Type u#x)
-  (r_in: parser)
-  (r_out:a -> parser)
-  (pre: pre_t r_in)
-  (post: post_t a r_in r_out pre)
-  (l: B.loc)
-  (spec: repr_spec a r_in r_out pre post)
-  (impl: repr_impl a r_in r_out pre post l spec)
-  ()
-: Write a r_in r_out pre post l
-= Write?.reflect (| spec, impl |)
+let valid_frame = admit ()
 
-
-assume
-val emp' : parser' unit
-
-let emp : parser = (| unit, emp' |)
-
-assume
-val valid_emp
-  (h: HS.mem)
-  (b: B.buffer u8)
-  (pos: U32.t)
-  (pos' : U32.t)
-: Lemma
-  (
-    valid_pos emp h b pos pos' <==> (
-    B.live h b /\
-    U32.v pos <= B.length b /\
-    U32.v pos' == U32.v pos
-  ))
-  [SMTPat (valid_pos emp h b pos pos')]
-
-assume
-val star' (#t1 #t2: Type) (p1: parser' t1) (p2: parser' t2) : Tot (parser' (t1 & t2))
-
-let star (p1 p2: parser) : Tot parser = (| (dfst p1 & dfst p2), star' (dsnd p1) (dsnd p2) |)
-
-assume
-val valid_star
-  (p1 p2: parser)
-  (h: HS.mem)
-  (b: B.buffer U8.t)
-  (pos1 pos2 pos3: U32.t)
-: Lemma
-  (requires (
-    valid_pos p1 h b pos1 pos2 /\
-    valid_pos p2 h b pos2 pos3
-  ))
-  (ensures (
-    valid_pos p1 h b pos1 pos2 /\
-    valid_pos p2 h b pos2 pos3 /\
-    valid_pos (p1 `star` p2) h b pos1 pos3 /\
-    contents (p1 `star` p2) h b pos1 pos3 == (contents p1 h b pos1 pos2, contents p2 h b pos2 pos3)
-  ))
-
-assume
-val valid_frame
-  (p: parser)
-  (h: HS.mem)
-  (b: B.buffer U8.t)
-  (pos: U32.t)
-  (pos' : U32.t)
-  (l: B.loc)
-  (h' : HS.mem)
-: Lemma
-  (requires (
-    valid_pos p h b pos pos' /\
-    B.modifies l h h' /\
-    B.loc_disjoint l (B.loc_buffer_from_to b pos pos')
-  ))
-  (ensures (
-    valid_pos p h b pos pos' /\
-    valid_pos p h' b pos pos' /\
-    contents p h' b pos pos' == contents p h b pos pos'
-  ))
-
-assume
-val valid_gsub
-  (p: parser)
-  (h: HS.mem)
-  (b: B.buffer U8.t)
-  (pos0 pos1 pos2: U32.t)
-  (len: U32.t)
-: Lemma
-  (requires (
-    U32.v pos0 + U32.v len <= B.length b /\
-    valid_pos p h (B.gsub b pos0 len) pos1 pos2
-  ))
-  (ensures (
-    U32.v pos0 + U32.v pos2 <= B.length b /\
-    valid_pos p h (B.gsub b pos0 len) pos1 pos2 /\
-    valid_pos p h b (pos0 `U32.add` pos1) (pos0 `U32.add` pos2) /\
-    contents p h b (pos0 `U32.add` pos1) (pos0 `U32.add` pos2) == contents p h (B.gsub b pos0 len) pos1 pos2
-  ))
-  [SMTPat (valid_pos p h (B.gsub b pos0 len) pos1 pos2)]
-
-let frame_out
-  (a: Type)
-  (frame: parser)
-  (p: (a -> Tot parser))
-  (x: a)
-: Tot parser
-= frame `star` (p x)
-
-unfold
-let frame_pre
-  (a: Type)
-  (frame: parser)
-  (pre: pre_t emp)
-: Tot (pre_t frame)
-= fun _ -> pre ()
-
-unfold
-let frame_post
-  (a: Type)
-  (frame: parser)
-  (pre: pre_t emp)
-  (p: a -> parser)
-  (post: post_t a emp p pre)
-: Tot (post_t a frame (frame_out a frame p) (frame_pre a frame pre))
-= fun v_in v (v_in', v_out) -> v_in == v_in' /\ post () v v_out
-
-let frame_spec
-  (a: Type)
-  (frame: parser)
-  (pre: pre_t emp)
-  (p: a -> parser)
-  (post: post_t a emp p pre)
-  (l: B.loc)
-  (inner: unit -> Write a emp p pre post l)
-: Tot (repr_spec a frame (frame_out a frame p) (frame_pre a frame pre) (frame_post a frame pre p post))
-= fun fr ->
-  let (| v, w |) = destr_repr_spec a emp p pre post l inner () in
-  (| v, (fr, w) |)
+let valid_gsub = admit ()
 
 inline_for_extraction
 let frame_impl
@@ -568,69 +182,18 @@ let frame_impl
   valid_star frame (p x) h' buf 0ul pos pos' ;
   (x, pos')
 
-inline_for_extraction
-let frame'
-  (a: Type)
-  (frame: parser)
-  (pre: pre_t emp)
-  (p: a -> parser)
-  (post: post_t a emp p pre)
-  (l: B.loc)
-  (inner: unit -> Write a emp p pre post l)
-: Tot (unit -> Write a frame (frame_out a frame p) (frame_pre a frame pre) (frame_post a frame pre p post) l)
-= mk_repr
-    a frame (frame_out a frame p) (frame_pre a frame pre) (frame_post a frame pre p post) l
-    (frame_spec a frame pre p post l inner)
-    (frame_impl a frame pre p post l inner)
+let parse_u32' = admit ()
+
+let write_u32 = admit ()
 
 inline_for_extraction
-let frame
-  (a: Type)
-  (frame: parser)
-  (pre: pre_t emp)
-  (p: a -> parser)
-  (post: post_t a emp p pre)
+let recast_writer_impl
+  (a:Type u#x)
+  (r_in: parser)
+  (r_out:a -> parser)
+  (pre: pre_t r_in)
+  (post: post_t a r_in r_out pre)
   (l: B.loc)
-  (inner: unit -> Write a emp p pre post l)
-: Write a frame (frame_out a frame p) (frame_pre a frame pre) (frame_post a frame pre p post) l
-= frame' a frame pre p post l inner ()
-
-let elem_writer
-  (p: parser)
-: Tot Type
-= (#l: B.loc) -> (x: dfst p) -> Write unit emp (fun _ -> p) (fun _ -> True) (fun _ _ y -> y == x) l
-
-let append
-  (#fr: parser)
-  (#p: parser)
-  (w: elem_writer p)
-  (#l: B.loc)
-  (x: dfst p)
-: Write unit fr (fun _ -> fr `star` p) (fun _ -> True) (fun w _ (w', x') -> w' == w /\ x' == x) l
-= frame unit fr (fun _ -> True) (fun _ -> p) (fun _ _ x' -> x' == x) l (fun _ -> w x)
-
-assume
-val parse_u32' : parser' U32.t
-
-let parse_u32 : parser = (| U32.t , parse_u32' |)
-
-assume
-val write_u32 : elem_writer parse_u32
-
-let write_two_ints
-  (l: B.loc)
-  (x y: U32.t)
-: Write unit emp (fun _ -> parse_u32 `star` parse_u32) (fun _ -> True) (fun _ _ (x', y') -> x' == x /\ y' == y) l
-= write_u32 x;
-  append write_u32 y
-
-let write_two_ints_ifthenelse
-  (l: B.loc)
-  (x y: U32.t)
-: Write unit emp (fun _ -> parse_u32 `star` parse_u32) (fun _ -> True) (fun _ _ (x', y') -> x' == x /\ y' == (if U32.v x < U32.v y then x else y)) l
-= write_u32 x;
-  if x `U32.lt` y
-  then
-    append write_u32 x
-  else
-    append write_u32 y
+  (f: unit -> Write a r_in r_out pre post l)
+: Tot (repr_impl a r_in r_out pre (recast_writer_post a r_in r_out pre post l f) l (recast_writer_spec a r_in r_out pre post l f))
+= fun b pos -> destr_repr_impl a r_in r_out pre post l f b pos
