examples/layeredeffects/LowParseWriters.fsti
@@ -1,0 +1,705 @@
+(*
+   Copyright 2019 Microsoft Research
+
+   Licensed under the Apache License, Version 2.0 (the "License");
+   you may not use this file except in compliance with the License.
+   You may obtain a copy of the License at
+
+       http://www.apache.org/licenses/LICENSE-2.0
+
+   Unless required by applicable law or agreed to in writing, software
+   distributed under the License is distributed on an "AS IS" BASIS,
+   WITHOUT WARRANTIES OR CONDITIONS OF ANY KIND, either express or implied.
+   See the License for the specific language governing permissions and
+   limitations under the License.
+*)
+
+module LowParseWriters
+
+
+open FStar.HyperStack.ST
+
+module HS = FStar.HyperStack
+module B = LowStar.Buffer
+module U8 = FStar.UInt8
+module U32 = FStar.UInt32
+module HST = FStar.HyperStack.ST
+
+val parser' (t: Type0) : Type0
+
+let parser : Type u#1 = (t: Type0 & parser' t)
+
+inline_for_extraction
+let dsnd
+  (#u: Type)
+  (#v: ((x: u) -> Type))
+  (p: dtuple2 u v)
+: Tot (v (dfst p))
+= match p with (| _, x |) -> x
+
+val valid_pos
+  (p: parser)
+  (h: HS.mem)
+  (b: B.buffer U8.t)
+  (pos: U32.t)
+  (pos' : U32.t)
+: GTot Type0
+
+val valid_pos_post
+  (p: parser)
+  (h: HS.mem)
+  (b: B.buffer U8.t)
+  (pos: U32.t)
+  (pos' : U32.t)
+: Lemma
+  (requires (valid_pos p h b pos pos'))
+  (ensures (
+    B.live h b /\
+    U32.v pos <= U32.v pos' /\
+    U32.v pos' <= B.length b
+  ))
+  [SMTPat (valid_pos p h b pos pos')]
+
+val contents
+  (p: parser)
+  (h: HS.mem)
+  (b: B.buffer U8.t)
+  (pos: U32.t)
+  (pos' : U32.t)
+: Ghost (dfst p)
+  (requires (valid_pos p h b pos pos'))
+  (ensures (fun _ -> True))
+
+unfold
+let pure_wp_mono
+  (a: Type)
+  (wp: pure_wp a)
+: GTot Type0
+= (forall (p q:pure_post a).
+     (forall (x:a). p x ==> q x) ==> (wp p ==> wp q))
+
+let pre_t
+  (rin: parser)
+: Tot Type
+= dfst rin -> GTot Type0
+
+let post_t
+  (a: Type)
+  (rin: parser)
+  (rout: a -> Tot parser)
+  (pre: pre_t rin)
+: Tot Type
+= (x: dfst rin { pre x }) -> (res: a) -> dfst (rout res) -> GTot Type0
+
+inline_for_extraction
+let repr_spec (a:Type u#x) (r_in: parser) (r_out:a -> parser) (pre: pre_t r_in) (post: post_t a r_in r_out pre) : Tot (Type u#x) =
+  (v_in: dfst r_in) ->
+  Ghost (v: a & dfst (r_out v))
+  (requires (pre v_in))
+  (ensures (fun (| v, v_out |) -> post v_in v v_out))
+
+type u8 : Type0 = U8.t
+
+inline_for_extraction
+val repr_impl
+  (a:Type u#x)
+  (r_in: parser)
+  (r_out:a -> parser)
+  (pre: pre_t r_in)
+  (post: post_t a r_in r_out pre)
+  (l: B.loc)
+  (spec: repr_spec a r_in r_out pre post)
+: Tot Type0
+
+inline_for_extraction
+let repr
+  (a: Type u#x)
+  (r_in: parser) (r_out:a -> parser)
+  (pre: pre_t r_in)
+  (post: post_t a r_in r_out pre)
+  (l: B.loc)
+: Tot (Type u#x)
+= dtuple2 (repr_spec a r_in r_out pre post) (repr_impl a r_in r_out pre post l)
+
+// unfold
+let return_pre
+  (a:Type) (x:a) (r: a -> parser)
+: Tot (pre_t (r x))
+= fun _ -> True
+
+// unfold
+let return_post
+  (a:Type) (x:a) (r: a -> parser)
+: Tot (post_t a (r x) r (return_pre a x r))
+= fun ppre x' ppost -> x' == x /\ ppost == ppre
+
+let return_spec
+  (a:Type) (x:a) (r: a -> parser)
+: Tot (repr_spec a (r x) r (return_pre a x r) (return_post a x r))
+= fun c -> (| x, c |)
+
+inline_for_extraction
+val return_impl
+  (a:Type) (x:a) (r: a -> parser)
+  (l: B.loc)
+: Tot (repr_impl a (r x) r (return_pre a x r) (return_post a x r) l (return_spec a x r))
+
+inline_for_extraction
+let returnc
+  (a:Type) (x:a) (r: a -> parser) (l: B.loc)
+: Tot (repr a (r x) r (return_pre a x r) (return_post a x r) l)
+= (| return_spec a x r, return_impl a x r l |)
+
+let bind_pre
+  (a:Type) (b:Type)
+  (r_in_f:parser) (r_out_f:a -> parser)
+  (pre_f:pre_t r_in_f) (post_f: post_t a r_in_f r_out_f pre_f)
+  (pre_g: (x:a) ->  pre_t (r_out_f x))
+: Tot (pre_t r_in_f)
+= fun v_in -> pre_f v_in /\ (forall (x: a) v_out . post_f v_in x v_out ==> pre_g x v_out)
+
+let bind_post
+  (a:Type) (b:Type)
+  (r_in_f:parser) (r_out_f:a -> parser)
+  (pre_f:pre_t r_in_f) (post_f: post_t a r_in_f r_out_f pre_f)
+  (r_out_g:b -> parser)
+  (pre_g: (x:a) ->  pre_t (r_out_f x))
+  (post_g: (x:a) -> post_t b (r_out_f x) r_out_g (pre_g x))
+: Tot (post_t b r_in_f r_out_g (bind_pre a b r_in_f r_out_f pre_f post_f pre_g))
+= fun v_in y v_out ->
+  exists x v_out_f . pre_f v_in /\ post_f v_in x v_out_f /\ post_g x v_out_f y v_out
+
+let bind_spec (a:Type) (b:Type)
+  (r_in_f:parser) (r_out_f:a -> parser)
+  (pre_f: pre_t r_in_f) (post_f: post_t a r_in_f r_out_f pre_f)
+  (r_out_g:b -> parser)
+  (pre_g: (x:a) -> pre_t (r_out_f x)) (post_g: (x:a) -> post_t b (r_out_f x) r_out_g (pre_g x))
+  (f_bind_spec:repr_spec a r_in_f r_out_f pre_f post_f)
+  (g:(x:a -> repr_spec b (r_out_f x) r_out_g (pre_g x) (post_g x)))
+: Tot (repr_spec b r_in_f r_out_g (bind_pre a b r_in_f r_out_f pre_f post_f pre_g) (bind_post a b r_in_f r_out_f pre_f post_f r_out_g pre_g post_g))
+= fun c ->
+  match f_bind_spec c with
+  | (| x, cf |) ->
+    g x cf
+
+inline_for_extraction
+val bind_impl
+  (a:Type) (b:Type)
+  (r_in_f:parser) (r_out_f:a -> parser)
+  (pre_f: pre_t r_in_f) (post_f: post_t a r_in_f r_out_f pre_f)
+  (r_out_g:b -> parser)
+  (pre_g: (x:a) -> pre_t (r_out_f x)) (post_g: (x:a) -> post_t b (r_out_f x) r_out_g (pre_g x))
+  (f_bind_impl:repr_spec a r_in_f r_out_f pre_f post_f)
+  (g:(x:a -> repr_spec b (r_out_f x) r_out_g (pre_g x) (post_g x)))
+  (l: B.loc)
+  (f' : repr_impl a r_in_f r_out_f pre_f post_f l f_bind_impl)
+  (g' : (x: a -> repr_impl b (r_out_f x) r_out_g (pre_g x) (post_g x) l (g x)))
+: Tot (repr_impl b r_in_f r_out_g (bind_pre a b r_in_f r_out_f pre_f post_f pre_g) (bind_post a b r_in_f r_out_f pre_f post_f r_out_g pre_g post_g) l (bind_spec a b r_in_f r_out_f pre_f post_f r_out_g pre_g post_g f_bind_impl g))
+
+inline_for_extraction
+let bind (a:Type) (b:Type)
+  (r_in_f:parser) (r_out_f:a -> parser)
+  (pre_f: pre_t r_in_f) (post_f: post_t a r_in_f r_out_f pre_f)
+  (r_out_g:b -> parser)
+  (pre_g: (x:a) -> pre_t (r_out_f x)) (post_g: (x:a) -> post_t b (r_out_f x) r_out_g (pre_g x))
+  (l: B.loc)
+  (f_bind : repr a r_in_f r_out_f pre_f post_f l)
+  (g : (x: a -> repr b (r_out_f x) r_out_g (pre_g x) (post_g x) l))
+: Tot (repr b r_in_f r_out_g (bind_pre a b r_in_f r_out_f pre_f post_f pre_g) (bind_post a b r_in_f r_out_f pre_f post_f r_out_g pre_g post_g) l)
+= (| bind_spec a b r_in_f r_out_f pre_f post_f r_out_g pre_g post_g (dfst f_bind) (fun x -> dfst (g x)), bind_impl a b r_in_f r_out_f pre_f post_f r_out_g pre_g post_g (dfst f_bind) (fun x -> dfst (g x)) l (dsnd f_bind) (fun x -> dsnd (g x)) |)
+
+unfold
+let subcomp_spec_cond
+  (a:Type)
+  (r_in:parser) (r_out:a -> parser)
+  (pre: pre_t r_in) (post: post_t a r_in r_out pre)
+  (pre': pre_t r_in) (post': post_t a r_in r_out pre')
+: GTot Type0
+= (forall v_in . pre' v_in ==> pre v_in) /\
+  (forall v_in x v_out . (pre' v_in /\ post v_in x v_out) ==> post' v_in x v_out)
+
+unfold
+let subcomp_cond
+  (a:Type)
+  (r_in:parser) (r_out:a -> parser)
+  (pre: pre_t r_in) (post: post_t a r_in r_out pre)
+  (pre': pre_t r_in) (post': post_t a r_in r_out pre')
+  (l:B.loc)
+  (l' : B.loc)
+: GTot Type0
+= l `B.loc_includes` l' /\
+  subcomp_spec_cond a r_in r_out pre post pre' post'
+
+let subcomp_spec (a:Type)
+  (r_in:parser) (r_out:a -> parser)
+  (pre: pre_t r_in) (post: post_t a r_in r_out pre)
+  (pre': pre_t r_in) (post': post_t a r_in r_out pre')
+  (f_subcomp:repr_spec a r_in r_out pre post)
+: Pure (repr_spec a r_in r_out pre' post')
+  (requires (subcomp_spec_cond a r_in r_out pre post pre' post'))
+  (ensures (fun _ -> True))
+= (fun x -> f_subcomp x)
+
+inline_for_extraction
+val subcomp_impl (a:Type)
+  (r_in:parser) (r_out:a -> parser)
+  (pre: pre_t r_in) (post: post_t a r_in r_out pre)
+  (pre': pre_t r_in) (post': post_t a r_in r_out pre')
+  (l:B.loc)
+  (l' : B.loc)
+  (f_subcomp_spec:repr_spec a r_in r_out pre post)
+  (f_subcomp:repr_impl a r_in r_out pre post l f_subcomp_spec)
+  (sq: squash (subcomp_cond a r_in r_out pre post pre' post' l l'))
+: Tot (repr_impl a r_in r_out pre' post' l' (subcomp_spec a r_in r_out pre post pre' post' f_subcomp_spec))
+
+inline_for_extraction
+let subcomp (a:Type)
+  (r_in:parser) (r_out:a -> parser)
+  (pre: pre_t r_in) (post: post_t a r_in r_out pre)
+  (pre': pre_t r_in) (post': post_t a r_in r_out pre')
+  (l:B.loc)
+  (l' : B.loc)
+  (f_subcomp:repr a r_in r_out pre post l)
+: Pure (repr a r_in r_out pre' post' l')
+  (requires (subcomp_cond a r_in r_out pre post pre' post' l l'))
+  (ensures (fun _ -> True))
+= (| subcomp_spec a r_in r_out pre post pre' post' (dfst f_subcomp),
+     subcomp_impl a r_in r_out pre post pre' post' l l' (dfst f_subcomp) (dsnd f_subcomp) ()
+  |)
+
+let if_then_else_pre
+  (r_in:parser)
+  (pre_f pre_g: pre_t r_in)
+  (p:Type0)
+: Tot (pre_t r_in)
+= fun v_in -> (p ==> pre_f v_in) /\ ((~ p) ==> pre_g v_in)
+
+let if_then_else_post
+  (a:Type)
+  (r_in:parser) (r_out:a -> parser)
+  (pre_f pre_g: pre_t r_in)
+  (post_f: post_t a r_in r_out pre_f)
+  (post_g: post_t a r_in r_out pre_g)
+  (p:Type0)
+: Tot (post_t a r_in r_out (if_then_else_pre r_in pre_f pre_g p))
+= fun v_in x v_out ->
+  (p ==> post_f v_in x v_out) /\
+  ((~ p) ==> post_g v_in x v_out)
+
+let if_then_else (a:Type)
+  (r_in:parser) (r_out:a -> parser)
+  (pre_f pre_g: pre_t r_in)
+  (post_f: post_t a r_in r_out pre_f)
+  (post_g: post_t a r_in r_out pre_g)
+  (l:B.loc)
+  (f_ifthenelse:repr a r_in r_out pre_f post_f l)
+  (g:repr a r_in r_out pre_g post_g l)
+  (p:Type0)
+: Tot Type
+= repr a r_in r_out (if_then_else_pre r_in pre_f pre_g p) (if_then_else_post a r_in r_out pre_f pre_g post_f post_g p) l
+
+reifiable reflectable total
+layered_effect {
+  Write : a:Type -> (pin: parser) -> (pout: (a -> parser)) -> (pre: pre_t pin) -> (post: post_t a pin pout pre) -> (B.loc) -> Effect
+  with
+  repr = repr;
+  return = returnc;
+  bind = bind;
+  subcomp = subcomp;
+  if_then_else = if_then_else
+}
+
+unfold
+let lift_pure_pre
+  (a:Type) (wp:pure_wp a { pure_wp_mono a wp }) (r:parser)
+: Tot (pre_t r)
+= fun st -> wp (fun _ -> True)
+
+unfold
+let lift_pure_post
+  (a:Type) (wp:pure_wp a { pure_wp_mono a wp }) (r:parser)
+: Tot (post_t a r (fun _ -> r) (lift_pure_pre a wp r))
+= fun st x st' -> ~ (wp (fun x' -> ~ (st == st' /\ x == x')))
+
+let lift_pure_spec
+  (a:Type) (wp:pure_wp a { pure_wp_mono a wp }) (r:parser) (f_pure_spec:unit -> PURE a wp)
+: Tot (repr_spec a r (fun _ -> r) (lift_pure_pre a wp r) (lift_pure_post a wp r))
+= fun v -> (| f_pure_spec (), v |)
+
+inline_for_extraction
+val lift_pure_impl
+  (a:Type) (wp:pure_wp a { pure_wp_mono a wp }) (r:parser) (f_pure_spec_for_impl:unit -> PURE a wp)
+  (l: B.loc)
+: Tot (repr_impl a r (fun _ -> r)  (fun v_in -> lift_pure_pre a wp r v_in) (fun v_in x v_out -> lift_pure_post a wp r v_in x v_out) l (lift_pure_spec a wp r f_pure_spec_for_impl))
+
+inline_for_extraction
+let lift_pure (a:Type) (wp:pure_wp a { pure_wp_mono a wp }) (r:parser)
+  (l: B.loc)
+  (f_pure:unit -> PURE a wp)
+: Tot (repr a r (fun _ -> r) (fun v_in -> lift_pure_pre a wp r v_in) (fun v_in x v_out -> lift_pure_post a wp r v_in x v_out) l)
+= (| lift_pure_spec a wp r f_pure, lift_pure_impl a wp r f_pure l |)
+
+sub_effect PURE ~> Write = lift_pure
+
+unfold
+let destr_repr_spec
+  (a:Type u#x)
+  (r_in: parser)
+  (r_out:a -> parser)
+  (pre: pre_t r_in)
+  (post: post_t a r_in r_out pre)
+  (l: B.loc)
+  ($f_destr_spec: unit -> Write a r_in r_out pre post l)
+: Tot (repr_spec a r_in r_out pre post)
+= dfst (reify (f_destr_spec ()))
+
+inline_for_extraction
+let destr_repr_impl
+  (a:Type u#x)
+  (r_in: parser)
+  (r_out:a -> parser)
+  (pre: pre_t r_in)
+  (post: post_t a r_in r_out pre)
+  (l: B.loc)
+  (f_destr_spec: unit -> Write a r_in r_out pre post l)
+: Tot (repr_impl a r_in r_out pre post l (destr_repr_spec a r_in r_out pre post l f_destr_spec))
+= dsnd (reify (f_destr_spec ()))
+
+inline_for_extraction
+unfold
+let mk_repr
+  (a:Type u#x)
+  (r_in: parser)
+  (r_out:a -> parser)
+  (pre: pre_t r_in)
+  (post: post_t a r_in r_out pre)
+  (l: B.loc)
+  (spec: repr_spec a r_in r_out pre post)
+  (impl: repr_impl a r_in r_out pre post l spec)
+  ()
+: Write a r_in r_out pre post l
+= Write?.reflect (| spec, impl |)
+
+val emp' : parser' unit
+
+let emp : parser = (| unit, emp' |)
+
+val valid_emp
+  (h: HS.mem)
+  (b: B.buffer u8)
+  (pos: U32.t)
+  (pos' : U32.t)
+: Lemma
+  (
+    valid_pos emp h b pos pos' <==> (
+    B.live h b /\
+    U32.v pos <= B.length b /\
+    U32.v pos' == U32.v pos
+  ))
+  [SMTPat (valid_pos emp h b pos pos')]
+
+val star' (#t1 #t2: Type) (p1: parser' t1) (p2: parser' t2) : Tot (parser' (t1 & t2))
+
+let star (p1 p2: parser) : Tot parser = (| (dfst p1 & dfst p2), star' (dsnd p1) (dsnd p2) |)
+
+val valid_star
+  (p1 p2: parser)
+  (h: HS.mem)
+  (b: B.buffer U8.t)
+  (pos1 pos2 pos3: U32.t)
+: Lemma
+  (requires (
+    valid_pos p1 h b pos1 pos2 /\
+    valid_pos p2 h b pos2 pos3
+  ))
+  (ensures (
+    valid_pos p1 h b pos1 pos2 /\
+    valid_pos p2 h b pos2 pos3 /\
+    valid_pos (p1 `star` p2) h b pos1 pos3 /\
+    contents (p1 `star` p2) h b pos1 pos3 == (contents p1 h b pos1 pos2, contents p2 h b pos2 pos3)
+  ))
+
+val valid_frame
+  (p: parser)
+  (h: HS.mem)
+  (b: B.buffer U8.t)
+  (pos: U32.t)
+  (pos' : U32.t)
+  (l: B.loc)
+  (h' : HS.mem)
+: Lemma
+  (requires (
+    valid_pos p h b pos pos' /\
+    B.modifies l h h' /\
+    B.loc_disjoint l (B.loc_buffer_from_to b pos pos')
+  ))
+  (ensures (
+    valid_pos p h b pos pos' /\
+    valid_pos p h' b pos pos' /\
+    contents p h' b pos pos' == contents p h b pos pos'
+  ))
+
+val valid_gsub
+  (p: parser)
+  (h: HS.mem)
+  (b: B.buffer U8.t)
+  (pos0 pos1 pos2: U32.t)
+  (len: U32.t)
+: Lemma
+  (requires (
+    U32.v pos0 + U32.v len <= B.length b /\
+    valid_pos p h (B.gsub b pos0 len) pos1 pos2
+  ))
+  (ensures (
+    U32.v pos0 + U32.v pos2 <= B.length b /\
+    valid_pos p h (B.gsub b pos0 len) pos1 pos2 /\
+    valid_pos p h b (pos0 `U32.add` pos1) (pos0 `U32.add` pos2) /\
+    contents p h b (pos0 `U32.add` pos1) (pos0 `U32.add` pos2) == contents p h (B.gsub b pos0 len) pos1 pos2
+  ))
+  [SMTPat (valid_pos p h (B.gsub b pos0 len) pos1 pos2)]
+
+let frame_out
+  (a: Type)
+  (frame: parser)
+  (p: (a -> Tot parser))
+  (x: a)
+: Tot parser
+= frame `star` (p x)
+
+let frame_pre
+  (a: Type)
+  (frame: parser)
+  (pre: pre_t emp)
+: Tot (pre_t frame)
+= fun _ -> pre ()
+
+let frame_post
+  (a: Type)
+  (frame: parser)
+  (pre: pre_t emp)
+  (p: a -> parser)
+  (post: post_t a emp p pre)
+: Tot (post_t a frame (frame_out a frame p) (frame_pre a frame pre))
+= fun v_in v (v_in', v_out) -> v_in == v_in' /\ post () v v_out
+
+let frame_spec
+  (a: Type)
+  (frame: parser)
+  (pre: pre_t emp)
+  (p: a -> parser)
+  (post: post_t a emp p pre)
+  (l: B.loc)
+  (inner: unit -> Write a emp p pre post l)
+: Tot (repr_spec a frame (frame_out a frame p) (frame_pre a frame pre) (frame_post a frame pre p post))
+= fun fr ->
+  let (| v, w |) = destr_repr_spec a emp p pre post l inner () in
+  (| v, (fr, w) |)
+
+inline_for_extraction
+val frame_impl
+  (a: Type)
+  (frame: parser)
+  (pre: pre_t emp)
+  (p: a -> parser)
+  (post: post_t a emp p pre)
+  (l: B.loc)
+  (inner: unit -> Write a emp p pre post l)
+: Tot (repr_impl a frame (frame_out a frame p) (frame_pre a frame pre) (frame_post a frame pre p post) l (frame_spec a frame pre p post l inner))
+
+inline_for_extraction
+let frame'
+  (a: Type)
+  (frame: parser)
+  (pre: pre_t emp)
+  (p: a -> parser)
+  (post: post_t a emp p pre)
+  (l: B.loc)
+  (inner: unit -> Write a emp p pre post l)
+: Tot (unit -> Write a frame (frame_out a frame p) (frame_pre a frame pre) (frame_post a frame pre p post) l)
+= mk_repr
+    a frame (frame_out a frame p) (frame_pre a frame pre) (frame_post a frame pre p post) l
+    (frame_spec a frame pre p post l inner)
+    (frame_impl a frame pre p post l inner)
+
+inline_for_extraction
+let frame
+  (a: Type)
+  (frame: parser)
+  (pre: pre_t emp)
+  (p: a -> parser)
+  (post: post_t a emp p pre)
+  (l: B.loc)
+  (inner: unit -> Write a emp p pre post l)
+: Write a frame (frame_out a frame p) (frame_pre a frame pre) (frame_post a frame pre p post) l
+= frame' a frame pre p post l inner ()
+
+let elem_writer_spec
+  (p: parser)
+  (x: dfst p)
+: Tot (repr_spec unit emp (fun _ -> p) (fun _ -> True) (fun _ _ y -> y == x))
+= fun _ -> (| (), x |)
+
+let elem_writer_impl_t
+  (p: parser)
+: Tot Type
+= (#l: B.loc) -> (x: dfst p) -> repr_impl unit emp (fun _ -> p) (fun _ -> True) (fun _ _ y -> y == x) l (elem_writer_spec p x)
+
+inline_for_extraction
+let start
+  (#p: parser)
+  (w: elem_writer_impl_t p)
+  (#l: B.loc)
+  (x: dfst p)
+: Write unit emp (fun _ -> p) (fun _ -> True) (fun _ _ y -> y == x) l
+= mk_repr
+    unit emp (fun _ -> p) (fun _ -> True) (fun _ _ y -> y == x) l
+    (elem_writer_spec p x)
+    (w x)
+    ()
+
+let append
+  (#fr: parser)
+  (#p: parser)
+  (w: elem_writer_impl_t p)
+  (#l: B.loc)
+  (x: dfst p)
+: Write unit fr (fun _ -> fr `star` p) (fun _ -> True) (fun w _ (w', x') -> w' == w /\ x' == x) l
+= frame unit fr (fun _ -> True) (fun _ -> p) (fun _ _ x' -> x' == x) l (fun _ -> start w x)
+
+val parse_u32' : parser' U32.t
+
+let parse_u32 : parser = (| U32.t , parse_u32' |)
+
+val write_u32 : elem_writer_impl_t parse_u32
+
+let write_two_ints
+  (l: B.loc)
+  (x y: U32.t)
+: Write unit emp (fun _ -> parse_u32 `star` parse_u32) (fun _ -> True) (fun _ _ (x', y') -> x' == x /\ y' == y) l
+= start write_u32 x;
+  append write_u32 y
+
+let write_two_ints_2
+  (l: B.loc)
+  (x y: U32.t)
+  ()
+: Write unit emp (fun _ -> parse_u32 `star` parse_u32) (fun _ -> True) (fun _ _ _ -> True) l
+= start write_u32 x;
+  append write_u32 y
+
+[@@ expect_failure ] // FIXME: WHY WHY WHY?
+let write_two_ints_2_lemma_1
+  (l: B.loc)
+  (x y: U32.t)
+: Lemma
+  (destr_repr_spec unit emp (fun _ -> parse_u32 `star` parse_u32) (fun _ -> True) (fun _ _ _ -> True) l (write_two_ints_2 l x y) () == (| (), (x, y) |) )
+= ()
+
+[@@ expect_failure ] // FIXME: WHY WHY WHY?
+let write_two_ints_2_lemma_2
+  (l: B.loc)
+  (x y: U32.t)
+: Lemma
+  (True)
+= assert (dfst (reify (write_two_ints_2 l x y ())) () == (| (), (x, y) |))
+
+let write_two_ints_ifthenelse
+  (l: B.loc)
+  (x y: U32.t)
+: Write unit emp (fun _ -> parse_u32 `star` parse_u32) (fun _ -> True) (fun _ _ (x', y') -> x' == x /\ y' == (if U32.v x < U32.v y then x else y)) l
+= start write_u32 x;
+  if x `U32.lt` y
+  then
+    append write_u32 x
+  else
+    append write_u32 y
+
+let write_two_ints_ifthenelse_2_aux
+  (l: B.loc)
+  (x y: U32.t)
+  ()
+: Write unit emp (fun _ -> parse_u32 `star` parse_u32) (fun _ -> True) (fun _ _ _ -> True) l
+= start write_u32 x;
+  if x `U32.lt` y
+  then
+    append write_u32 x
+  else
+    append write_u32 y
+
+let write_two_ints_ifthenelse_2_aux_lemma
+  (l: B.loc)
+  (x y: U32.t)
+: Lemma
+  (destr_repr_spec unit emp (fun _ -> parse_u32 `star` parse_u32) (fun _ -> True) (fun _ _ _ -> True) l (write_two_ints_ifthenelse_2_aux l x y) () == (| (), (x, (if U32.v x < U32.v y then x else y)) |) )
+= admit () // FIXME: WHY WHY WHY?
+
+unfold
+let recast_writer_post
+  (a:Type u#x)
+  (r_in: parser)
+  (r_out:a -> parser)
+  (pre: pre_t r_in)
+  (post: post_t a r_in r_out pre)
+  (l: B.loc)
+  (f: unit -> Write a r_in r_out pre post l)
+: Tot (post_t a r_in r_out pre)
+=
+  fun v_in v v_out -> destr_repr_spec a r_in r_out pre post l f v_in == (| v, v_out |) /\ post v_in v v_out
+
+let recast_writer_spec
+  (a:Type u#x)
+  (r_in: parser)
+  (r_out:a -> parser)
+  (pre: pre_t r_in)
+  (post: post_t a r_in r_out pre)
+  (l: B.loc)
+  (f: unit -> Write a r_in r_out pre post l)
+: Tot (repr_spec a r_in r_out pre (recast_writer_post a r_in r_out pre post l f))
+= fun v_in -> destr_repr_spec a r_in r_out pre post l f v_in
+
+inline_for_extraction
+val recast_writer_impl
+  (a:Type u#x)
+  (r_in: parser)
+  (r_out:a -> parser)
+  (pre: pre_t r_in)
+  (post: post_t a r_in r_out pre)
+  (l: B.loc)
+  (f: unit -> Write a r_in r_out pre post l)
+: Tot (repr_impl a r_in r_out pre (recast_writer_post a r_in r_out pre post l f) l (recast_writer_spec a r_in r_out pre post l f))
+
+inline_for_extraction
+let recast_writer'
+  (a:Type u#x)
+  (r_in: parser)
+  (r_out:a -> parser)
+  (pre: pre_t r_in)
+  (post: post_t a r_in r_out pre)
+  (l: B.loc)
+  (f: unit -> Write a r_in r_out pre post l)
+: Tot (unit -> Write a r_in r_out pre (recast_writer_post a r_in r_out pre post l f) l)
+= mk_repr a r_in r_out pre (recast_writer_post a r_in r_out pre post l f) l
+    (recast_writer_spec a r_in r_out pre post l f)
+    (recast_writer_impl a r_in r_out pre post l f)
+
+inline_for_extraction
+let recast_writer
+  (a:Type u#x)
+  (r_in: parser)
+  (r_out:a -> parser)
+  (pre: pre_t r_in)
+  (post: post_t a r_in r_out pre)
+  (l: B.loc)
+  ($f: unit -> Write a r_in r_out pre post l)
+: Write a r_in r_out pre (recast_writer_post a r_in r_out pre post l f) l
+= recast_writer' a r_in r_out pre post l f ()
+
+let write_two_ints_ifthenelse_2
+  (l: B.loc)
+  (x y: U32.t)
+: Write unit emp (fun _ -> parse_u32 `star` parse_u32)
+    (fun _ -> True)
+    (fun _ _ (x', y') -> x' == x /\ y' == (if U32.v x < U32.v y then x else y))
+    l
+= write_two_ints_ifthenelse_2_aux_lemma l x y;
+  recast_writer _ _ _ _ _ _ (write_two_ints_ifthenelse_2_aux l x y)
